Add derived patterns for EDTL requirements

examples/Constrained_Until.thy
@@ -63,75 +63,73 @@ toEnvP s \<Longrightarrow>A2' s s \<or> A1' s s \<and> t1 s > 0 \<Longrightarrow
   unfolding constrained_until_inv_def always_imp_def
   by (metis bot_nat_0.extremum dual_order.refl leD order_le_imp_less_or_eq toEnvNum_id)
 
-definition P1 where "P1 t A1 A2 A3 s \<equiv> 
-always  (\<lambda> r2 r1.  \<not> A1 r1 \<or> constrained_until t A2 A3 r2 r1) s"
+definition constrained_until2 where "constrained_until2 t1 t2 A1 A2  s s1 \<equiv>
+toEnvNum s1 s \<ge> t2 \<longrightarrow>
+(\<exists> r2. toEnvP r2 \<and> s1 \<le> r2 \<and> r2 \<le> s \<and> toEnvNum s1 r2 \<ge> t1 \<and> toEnvNum s1 r2 \<le> t2 \<and> A2 s r2 \<and>
+(\<forall> r1. toEnvP r1 \<and> s1 \<le> r1 \<and> r1 < r2 \<longrightarrow> A1 s r1))"
 
-definition P1_inv where "P1_inv t t1 A1 A2' A3' s \<equiv> 
-always_inv (\<lambda> r2 r1.  \<not> A1 r1 \<or> constrained_until_inv t t1 A2' A3' r2 r1) s"
+definition constrained_until2_inv where "constrained_until2_inv  t1 t2 t1_1 t2_1 A1' A2' s s1 \<equiv>
+(\<exists> r2. toEnvP r2 \<and> s1 \<le> r2 \<and> r2 \<le> s \<and> toEnvNum s1 r2 \<ge> t1 \<and> toEnvNum s1 r2 \<le> t2 \<and> A2' s r2 \<and>
+(\<forall> r1. toEnvP r1 \<and> s1 \<le> r1 \<and> r1 < r2 \<longrightarrow> A1' s r1)) \<or>
+toEnvNum s1 s \<ge> t1_1 s \<and> toEnvNum s1 s < t2_1 s \<and>
+(\<forall> r1. toEnvP r1 \<and> s1 \<le> r1 \<and> r1 \<le> s \<longrightarrow> A1' s r1)"
 
-lemma P1'inv_rule_gen: "
- P1_inv t t1 A1 A2' A3' s \<Longrightarrow> consecutive s s' \<Longrightarrow>
-(always_imp s (\<lambda>s1. \<not> A1 s1) (\<lambda>s1. \<not> A1 s1) \<and>  always_imp s (A2' s) (A2' s') \<and>
-    always_imp s (A3' s) (A3' s') \<and> (t1 s = STOP \<or> A3' s' s' \<and> t1 s \<le> t \<or> A2' s' s' \<and> t1 s < t1 s')) \<and>
- (\<not> A1 s' \<or> A3' s' s' \<or> A2' s' s' \<and> STOP < t1 s') \<Longrightarrow>
- P1_inv t t1 A1 A2' A3'  s'"
-  unfolding P1_inv_def
-  apply proveOuter
-  done
- (* apply(erule elims)
-   apply assumption
-  apply(erule conjE)
-  subgoal premises prems1
-    apply(rule conjI)
-     apply(insert prems1(1,2))[1]
-     apply(rule patternintro)
-      apply simp
-     apply(erule conjE)
-    subgoal premises prems2
-      apply(rule conjI)
-       apply(insert prems2(1,2))[1]
-       apply assumption
-      apply(insert prems2(1,3))
-      apply(rule patternintro)
-       apply assumption
-      apply assumption
-      done
-    apply(insert prems1(1,3))
+lemma constrained_until2_rule: "
+consecutive s s' \<Longrightarrow>
+always_imp s (A1' s) (A1' s') \<and>
+always_imp s (A2' s) (A2' s') \<and>
+ (t2_1 s = 0 \<or> t1_1 s \<ge> t2_1 s \<or> A2' s' s' \<and> t1_1 s + 1 \<ge> t1 \<and> t2_1 s \<le> t2 \<or> A1' s' s' \<and> t1_1 s + 1 \<ge> t1_1 s' \<and> t2_1 s < t2_1 s') \<Longrightarrow>
+always_imp s (\<lambda> s1. constrained_until2_inv t1 t2 t1_1 t2_1 A1' A2' s s1) (\<lambda> s1. constrained_until2_inv t1 t2 t1_1 t2_1 A1' A2' s' s1)"
+  apply(unfold constrained_until2_inv_def always_imp_def)
+    unfolding less_eq_state.simps less_state.simps
+    apply(rule allI)
+  subgoal for s1
+    apply(rule impI)
+    apply(erule conjE)+
+    apply(rotate_tac -1)
+    apply(erule disjE)
+     apply (metis consecutive.simps substate_trans)
+    apply(erule disjE)
+     apply simp
+    apply(erule disjE)
+     apply simp
     apply(erule disjE)
      apply(rule disjI1)
-     apply assumption
+     apply(rule exI[of _ s'])
+     apply(rule conjI)
+      apply simp
+     apply(rule conjI)
+      apply simp
+      apply (meson substate_trans)
+     apply(rule conjI)
+      apply simp
+     apply(rule conjI)
+    using toEnvNum3 apply auto[1]
+     apply(rule conjI)
+    using toEnvNum3 apply auto[1]
+     apply (metis consecutive.elims(2) substate_noteq_imp_substate_of_pred)
     apply(rule disjI2)
-    apply(rule patternintro)
-     apply simp
-    apply assumption
-    done
-  done
-*)
-
-lemma P1'inv_einv2req_gen: "
- P1_inv t t1 A1 A2' A3' s \<Longrightarrow> toEnvP s \<Longrightarrow>
-always_imp s (\<lambda>s1. \<not> A1 s1) (\<lambda>s1. \<not> A1 s1) \<and>  always_imp s (A2' s) (A2' s) \<and> always_imp s (A3' s) (A3' s) \<and> t1 s \<le> t
-  \<Longrightarrow>
- P1 t A1 A2' A3' s"
-  unfolding P1_inv_def P1_def
-  apply proveOuter
-  done
-(*  apply(erule elims)
-   apply assumption
-  apply(rule patternintro)
-   apply assumption
-  apply(erule conjE)
-  subgoal premises prems1
     apply(rule conjI)
-     apply(insert prems1(1,2))[1]
-     apply assumption
-    apply(insert prems1(1,3))
-    apply(rule patternintro)
-     apply assumption
-    apply assumption
-    done
+    using toEnvNum3 apply auto[1]
+    apply(rule conjI)
+    using toEnvNum3 apply auto[1]
+   using toEnvNum3
+    by (smt (verit, ccfv_SIG) consecutive.elims(2) less_imp_add_positive less_numeral_extra(3) less_one linorder_neqE_nat nat_add_left_cancel_less substate_noteq_imp_substate_of_pred trans_less_add1 zero_less_one)
   done
-*)
+
+lemma constrained_until2_einv2req: "
+toEnvP s \<Longrightarrow>
+always_imp s (A1' s) (A1 s) \<and>
+always_imp s (A2' s) (A2 s) \<and>
+t2_1 s \<le> t2 \<Longrightarrow>
+always_imp s (\<lambda> s1. constrained_until2_inv t1 t2 t1_1 t2_1 A1' A2' s s1) (\<lambda> s1. constrained_until2  t1 t2 A1 A2 s s1)"
+  unfolding constrained_until2_inv_def constrained_until2_def always_imp_def less_eq_state.simps less_state.simps
+  by (metis dual_order.trans substate_trans verit_comp_simplify1(3))
+
+lemma constrained_until2_one_point: "
+toEnvP s \<Longrightarrow>t1 = 0 \<and>A2' s s \<or> A1' s s \<and> t1_1 s = 0 \<and> t2_1 s > 0 \<Longrightarrow> constrained_until2_inv t1 t2 t1_1 t2_1 A1' A2' s s"
+  unfolding constrained_until2_inv_def always_imp_def
+ by (metis bot_nat_0.extremum dual_order.refl leD order_le_imp_less_or_eq toEnvNum_id)
 
 end
  
