examples/GasSeparator/EDTL_Patterns.thy
@@ -1,0 +1,1001 @@
+theory EDTL_Patterns imports VCProving.Basic_Patterns 
+begin
+
+definition EDTL_delay_true where "EDTL_delay_true trigger fin release Inv reaction s \<equiv> (always (\<lambda> r2 r1 . ((\<not> (trigger r1)) \<or> ((release r2 r1) \<or> (weak_until (\<lambda> r4 r3 . ((Inv r4 r3) \<and> (\<not> (fin r3)))) (\<lambda> r4 r3 . ((release r4 r3) \<or> ((fin r3) \<and> ((reaction r4 r3) \<and> (Inv r4 r3))))) r2 r1)))) s)"
+
+definition EDTL_delay_true_part where "EDTL_delay_true_part trigger fin release Inv reaction s \<equiv> (EDTL_delay_true trigger fin (\<lambda> s s1 . (release s1)) (\<lambda> s s1 . (Inv s1)) (\<lambda> s s1 . (reaction s1)) s)"
+
+definition EDTL_delay_true_inv where "EDTL_delay_true_inv w_0 trigger fin release_1 Inv_1 reaction_1 s \<equiv> (always_inv (\<lambda> r2 r1 . ((\<not> (trigger r1)) \<or> ((release_1 r2 r1) \<or> (weak_until_inv w_0 (\<lambda> r4 r3 . ((Inv_1 r4 r3) \<and> (\<not> (fin r3)))) (\<lambda> r4 r3 . ((release_1 r4 r3) \<or> ((fin r3) \<and> ((reaction_1 r4 r3) \<and> (Inv_1 r4 r3))))) r2 r1)))) s)"
+
+definition EDTL_delay_true_inv_part where "EDTL_delay_true_inv_part w_0 trigger fin release Inv reaction s \<equiv> (EDTL_delay_true_inv w_0 trigger fin (\<lambda> s s1 . (release s1)) (\<lambda> s s1 . (Inv s1)) (\<lambda> s s1 . (reaction s1)) s)"
+
+lemma EDTL_delay_true_inv_saving_gen: "
+EDTL_delay_true_inv w_0 trigger fin release_1 Inv_1 reaction_1 s0 \<Longrightarrow>
+consecutive s0 s \<Longrightarrow>
+((True \<and> ((always_imp s0 (\<lambda> r1 . (release_1 s0 r1)) (\<lambda> r1 . (release_1 s r1))) \<and> (((always_imp s0 (\<lambda> r3 . (Inv_1 s0 r3)) (\<lambda> r3 . (Inv_1 s r3))) \<and> True) \<and> (((always_imp s0 (\<lambda> r3 . (release_1 s0 r3)) (\<lambda> r3 . (release_1 s r3))) \<and> (True \<and> ((always_imp s0 (\<lambda> r3 . (reaction_1 s0 r3)) (\<lambda> r3 . (reaction_1 s r3))) \<and> (always_imp s0 (\<lambda> r3 . (Inv_1 s0 r3)) (\<lambda> r3 . (Inv_1 s r3)))))) \<and> ((\<not> (w_0 s0)) \<or> (((release_1 s s) \<or> ((fin s) \<and> ((reaction_1 s s) \<and> (Inv_1 s s)))) \<or> ((w_0 s) \<and> ((Inv_1 s s) \<and> (\<not> (fin s)))))))))) \<and> ((\<not> (trigger s)) \<or> ((release_1 s s) \<or> (((release_1 s s) \<or> ((fin s) \<and> ((reaction_1 s s) \<and> (Inv_1 s s)))) \<or> ((w_0 s) \<and> ((Inv_1 s s) \<and> (\<not> (fin s)))))))) \<Longrightarrow>
+EDTL_delay_true_inv w_0 trigger fin release_1 Inv_1 reaction_1 s"
+
+unfolding EDTL_delay_true_inv_def
+apply(erule always_rule)
+  apply simp
+  apply(erule conjE)
+  subgoal premises prems1
+  apply(rule conjI)
+  apply(insert prems1(1,2))[1]
+    apply(rule always_disj_rule)
+    apply simp
+      apply(erule conjE)
+      subgoal premises prems2
+      apply(rule conjI)
+      apply(insert prems2(1,2))[1]
+        apply(rule always_imp_refl)
+      apply(insert prems2(1,3))
+        apply(rule always_disj_rule)
+        apply simp
+          apply(erule conjE)
+          subgoal premises prems3
+          apply(rule conjI)
+          apply(insert prems3(1,2))[1]
+            apply simp
+          apply(insert prems3(1,3))
+            apply(rule weak_until_rule)
+            apply simp
+              apply(erule conjE)
+              subgoal premises prems4
+              apply(rule conjI)
+              apply(insert prems4(1,2))[1]
+                apply(rule always_conj_rule)
+                apply simp
+                  apply(erule conjE)
+                  subgoal premises prems5
+                  apply(rule conjI)
+                  apply(insert prems5(1,2))[1]
+                    apply simp
+                  apply(insert prems5(1,3))
+                    apply(rule always_imp_refl)
+                  done
+              apply(insert prems4(1,3))
+                apply(erule conjE)
+                subgoal premises prems6
+                apply(rule conjI)
+                apply(insert prems6(1,2))[1]
+                  apply(rule always_disj_rule)
+                  apply simp
+                    apply(erule conjE)
+                    subgoal premises prems7
+                    apply(rule conjI)
+                    apply(insert prems7(1,2))[1]
+                      apply simp
+                    apply(insert prems7(1,3))
+                      apply(rule always_conj_rule)
+                      apply simp
+                        apply(erule conjE)
+                        subgoal premises prems8
+                        apply(rule conjI)
+                        apply(insert prems8(1,2))[1]
+                          apply(rule always_imp_refl)
+                        apply(insert prems8(1,3))
+                          apply(rule always_conj_rule)
+                          apply simp
+                            apply(erule conjE)
+                            subgoal premises prems9
+                            apply(rule conjI)
+                            apply(insert prems9(1,2))[1]
+                              apply simp
+                            apply(insert prems9(1,3))
+                              apply simp
+                            done
+                        done
+                    done
+                apply(insert prems6(1,3))
+                  apply(erule disjE)
+                  apply(rule disjI1)
+                    apply simp
+                  apply(rule disjI2)
+                    apply(erule disjE)
+                    apply(rule disjI1)
+                      apply(erule disjE)
+                      apply(rule disjI1)
+                        apply simp
+                      apply(rule disjI2)
+                        apply(erule conjE)
+                        subgoal premises prems10
+                        apply(rule conjI)
+                        apply(insert prems10(1,2))[1]
+                          apply simp
+                        apply(insert prems10(1,3))
+                          apply(erule conjE)
+                          subgoal premises prems11
+                          apply(rule conjI)
+                          apply(insert prems11(1,2))[1]
+                            apply simp
+                          apply(insert prems11(1,3))
+                            apply simp
+                          done
+                        done
+                    apply(rule disjI2)
+                      apply(erule conjE)
+                      subgoal premises prems12
+                      apply(rule conjI)
+                      apply(insert prems12(1,2))[1]
+                        apply simp
+                      apply(insert prems12(1,3))
+                        apply(erule conjE)
+                        subgoal premises prems13
+                        apply(rule conjI)
+                        apply(insert prems13(1,2))[1]
+                          apply simp
+                        apply(insert prems13(1,3))
+                          apply simp
+                        done
+                      done
+                done
+              done
+          done
+      done
+  apply(insert prems1(1,3))
+    apply(erule disjE)
+    apply(rule disjI1)
+      apply simp
+    apply(rule disjI2)
+      apply(erule disjE)
+      apply(rule disjI1)
+        apply simp
+      apply(rule disjI2)
+        apply(rule weak_until_one_point)
+        apply simp
+          apply(erule disjE)
+          apply(rule disjI1)
+            apply(erule disjE)
+            apply(rule disjI1)
+              apply simp
+            apply(rule disjI2)
+              apply(erule conjE)
+              subgoal premises prems14
+              apply(rule conjI)
+              apply(insert prems14(1,2))[1]
+                apply simp
+              apply(insert prems14(1,3))
+                apply(erule conjE)
+                subgoal premises prems15
+                apply(rule conjI)
+                apply(insert prems15(1,2))[1]
+                  apply simp
+                apply(insert prems15(1,3))
+                  apply simp
+                done
+              done
+          apply(rule disjI2)
+            apply(erule conjE)
+            subgoal premises prems16
+            apply(rule conjI)
+            apply(insert prems16(1,2))[1]
+              apply simp
+            apply(insert prems16(1,3))
+              apply(erule conjE)
+              subgoal premises prems17
+              apply(rule conjI)
+              apply(insert prems17(1,2))[1]
+                apply simp
+              apply(insert prems17(1,3))
+                apply simp
+              done
+            done
+  done
+done
+
+lemma EDTL_delay_trueeinv_imp_req_gen: "
+EDTL_delay_true_inv w_0 trigger fin release_1 Inv_1 reaction_1 s0 \<Longrightarrow>
+toEnvP s0 \<Longrightarrow>
+(True \<and> ((always_imp s0 (\<lambda> r1 . (release_1 s0 r1)) (\<lambda> r1 . (release s0 r1))) \<and> (((always_imp s0 (\<lambda> r3 . (Inv_1 s0 r3)) (\<lambda> r3 . (Inv s0 r3))) \<and> True) \<and> ((always_imp s0 (\<lambda> r3 . (release_1 s0 r3)) (\<lambda> r3 . (release s0 r3))) \<and> (True \<and> ((always_imp s0 (\<lambda> r3 . (reaction_1 s0 r3)) (\<lambda> r3 . (reaction s0 r3))) \<and> (always_imp s0 (\<lambda> r3 . (Inv_1 s0 r3)) (\<lambda> r3 . (Inv s0 r3))))))))) \<Longrightarrow>
+EDTL_delay_true trigger fin release Inv reaction s0"
+
+unfolding EDTL_delay_true_inv_def EDTL_delay_true_def
+apply(erule always_einv2req)
+apply simp
+  apply(rule always_disj_rule)
+  apply simp
+    apply(erule conjE)
+    subgoal premises prems3
+    apply(rule conjI)
+    apply(insert prems3(1,2))[1]
+      apply(rule always_imp_refl)
+    apply(insert prems3(1,3))
+      apply(rule always_disj_rule)
+      apply simp
+        apply(erule conjE)
+        subgoal premises prems4
+        apply(rule conjI)
+        apply(insert prems4(1,2))[1]
+          apply simp
+        apply(insert prems4(1,3))
+          apply(rule weak_until_einv2req)
+          apply simp
+            apply(erule conjE)
+            subgoal premises prems5
+            apply(rule conjI)
+            apply(insert prems5(1,2))[1]
+              apply(rule always_conj_rule)
+              apply simp
+                apply(erule conjE)
+                subgoal premises prems6
+                apply(rule conjI)
+                apply(insert prems6(1,2))[1]
+                  apply simp
+                apply(insert prems6(1,3))
+                  apply(rule always_imp_refl)
+                done
+            apply(insert prems5(1,3))
+              apply(rule always_disj_rule)
+              apply simp
+                apply(erule conjE)
+                subgoal premises prems7
+                apply(rule conjI)
+                apply(insert prems7(1,2))[1]
+                  apply simp
+                apply(insert prems7(1,3))
+                  apply(rule always_conj_rule)
+                  apply simp
+                    apply(erule conjE)
+                    subgoal premises prems8
+                    apply(rule conjI)
+                    apply(insert prems8(1,2))[1]
+                      apply(rule always_imp_refl)
+                    apply(insert prems8(1,3))
+                      apply(rule always_conj_rule)
+                      apply simp
+                        apply(erule conjE)
+                        subgoal premises prems9
+                        apply(rule conjI)
+                        apply(insert prems9(1,2))[1]
+                          apply simp
+                        apply(insert prems9(1,3))
+                          apply simp
+                        done
+                    done
+                done
+            done
+        done
+    done
+done
+
+lemma EDTL_delay_true_inv_saving: "
+EDTL_delay_true_inv_part w_0 trigger fin release Inv reaction s0 \<Longrightarrow>
+consecutive s0 s \<Longrightarrow>
+(((\<not> (w_0 s0)) \<or> (((release s) \<or> ((fin s) \<and> ((reaction s) \<and> (Inv s)))) \<or> ((w_0 s) \<and> ((Inv s) \<and> (\<not> (fin s)))))) \<and> ((\<not> (trigger s)) \<or> ((release s) \<or> (((release s) \<or> ((fin s) \<and> ((reaction s) \<and> (Inv s)))) \<or> ((w_0 s) \<and> ((Inv s) \<and> (\<not> (fin s)))))))) \<Longrightarrow>
+EDTL_delay_true_inv_part w_0 trigger fin release Inv reaction s"
+
+unfolding EDTL_delay_true_inv_part_def EDTL_delay_true_part_def
+apply(simp add: EDTL_delay_true_inv_saving_gen always_imp_refl)
+done
+
+lemma EDTL_delay_trueeinv_imp_req: "
+EDTL_delay_true_inv_part w_0 trigger fin release Inv reaction s \<Longrightarrow>
+toEnvP s \<Longrightarrow>
+True \<Longrightarrow>
+EDTL_delay_true_part trigger fin release Inv reaction s"
+
+unfolding EDTL_delay_true_inv_part_def EDTL_delay_true_part_def
+apply(simp add: EDTL_delay_trueeinv_imp_req_gen always_imp_refl)
+done
+
+
+
+lemmas EDTL_delay_true_used_patterns = EDTL_delay_true_def always_used_patterns weak_until_def 
+
+lemmas EDTL_delay_true_inv_used_patterns = EDTL_delay_true_inv_def always_inv_used_patterns weak_until_inv_def 
+
+lemmas EDTL_delay_true_inv_part_used_patterns = EDTL_delay_true_inv_part_def EDTL_delay_true_inv_used_patterns
+
+lemmas EDTL_delay_true_part_used_patterns = EDTL_delay_true_part_def EDTL_delay_true_used_patterns
+
+definition EDTL_final_nontemporal_or_tau_delay_true where "EDTL_final_nontemporal_or_tau_delay_true finalt trigger finale release Inv reaction s \<equiv> (always (\<lambda> r2 r1 . ((\<not> (trigger r1)) \<or> ((release r2 r1) \<or> ((constrained_until finalt (\<lambda> r4 r3 . ((Inv r4 r3) \<and> (\<not> (finale r3)))) (\<lambda> r4 r3 . ((release r4 r3) \<or> ((finale r3) \<and> ((reaction r4 r3) \<and> (Inv r4 r3))))) r2 r1) \<or> (constrained_until2 finalt finalt (\<lambda> r4 r3 . ((Inv r4 r3) \<and> (\<not> (finale r3)))) (\<lambda> r4 r3 . ((reaction r4 r3) \<and> (Inv r4 r3))) r2 r1))))) s)"
+
+definition EDTL_final_nontemporal_or_tau_delay_true_part where "EDTL_final_nontemporal_or_tau_delay_true_part finalt trigger finale release Inv reaction s \<equiv> (EDTL_final_nontemporal_or_tau_delay_true finalt trigger finale (\<lambda> s s1 . (release s1)) (\<lambda> s s1 . (Inv s1)) (\<lambda> s s1 . (reaction s1)) s)"
+
+definition EDTL_final_nontemporal_or_tau_delay_true_inv where "EDTL_final_nontemporal_or_tau_delay_true_inv finalt t1_0 t1_1_0 t2_1_0 trigger finale release_1 Inv_1 reaction_1 s \<equiv> (always_inv (\<lambda> r2 r1 . ((\<not> (trigger r1)) \<or> ((release_1 r2 r1) \<or> ((constrained_until_inv finalt t1_0 (\<lambda> r4 r3 . ((Inv_1 r4 r3) \<and> (\<not> (finale r3)))) (\<lambda> r4 r3 . ((release_1 r4 r3) \<or> ((finale r3) \<and> ((reaction_1 r4 r3) \<and> (Inv_1 r4 r3))))) r2 r1) \<or> (constrained_until2_inv finalt finalt t1_1_0 t2_1_0 (\<lambda> r4 r3 . ((Inv_1 r4 r3) \<and> (\<not> (finale r3)))) (\<lambda> r4 r3 . ((reaction_1 r4 r3) \<and> (Inv_1 r4 r3))) r2 r1))))) s)"
+
+definition EDTL_final_nontemporal_or_tau_delay_true_inv_part where "EDTL_final_nontemporal_or_tau_delay_true_inv_part finalt t1_0 t1_1_0 t2_1_0 trigger finale release Inv reaction s \<equiv> (EDTL_final_nontemporal_or_tau_delay_true_inv finalt t1_0 t1_1_0 t2_1_0 trigger finale (\<lambda> s s1 . (release s1)) (\<lambda> s s1 . (Inv s1)) (\<lambda> s s1 . (reaction s1)) s)"
+
+lemma EDTL_final_nontemporal_or_tau_delay_true_inv_saving_gen: "
+EDTL_final_nontemporal_or_tau_delay_true_inv finalt t1_0 t1_1_0 t2_1_0 trigger finale release_1 Inv_1 reaction_1 s0 \<Longrightarrow>
+consecutive s0 s \<Longrightarrow>
+((True \<and> ((always_imp s0 (\<lambda> r1 . (release_1 s0 r1)) (\<lambda> r1 . (release_1 s r1))) \<and> ((((always_imp s0 (\<lambda> r3 . (Inv_1 s0 r3)) (\<lambda> r3 . (Inv_1 s r3))) \<and> True) \<and> (((always_imp s0 (\<lambda> r3 . (release_1 s0 r3)) (\<lambda> r3 . (release_1 s r3))) \<and> (True \<and> ((always_imp s0 (\<lambda> r3 . (reaction_1 s0 r3)) (\<lambda> r3 . (reaction_1 s r3))) \<and> (always_imp s0 (\<lambda> r3 . (Inv_1 s0 r3)) (\<lambda> r3 . (Inv_1 s r3)))))) \<and> (((t1_0 s0) = 0) \<or> ((((release_1 s s) \<or> ((finale s) \<and> ((reaction_1 s s) \<and> (Inv_1 s s)))) \<and> ((t1_0 s0) <= finalt)) \<or> (((Inv_1 s s) \<and> (\<not> (finale s))) \<and> ((t1_0 s0) < (t1_0 s))))))) \<and> (((always_imp s0 (\<lambda> r3 . (Inv_1 s0 r3)) (\<lambda> r3 . (Inv_1 s r3))) \<and> True) \<and> (((always_imp s0 (\<lambda> r3 . (reaction_1 s0 r3)) (\<lambda> r3 . (reaction_1 s r3))) \<and> (always_imp s0 (\<lambda> r3 . (Inv_1 s0 r3)) (\<lambda> r3 . (Inv_1 s r3)))) \<and> (((t2_1_0 s0) = 0) \<or> (((t1_1_0 s0) >= (t2_1_0 s0)) \<or> ((((reaction_1 s s) \<and> (Inv_1 s s)) \<and> ((((t1_1_0 s0) + 1) >= finalt) \<and> ((t2_1_0 s0) <= finalt))) \<or> (((Inv_1 s s) \<and> (\<not> (finale s))) \<and> ((((t1_1_0 s0) + 1) >= (t1_1_0 s)) \<and> ((t2_1_0 s0) < (t2_1_0 s)))))))))))) \<and> ((\<not> (trigger s)) \<or> ((release_1 s s) \<or> ((((release_1 s s) \<or> ((finale s) \<and> ((reaction_1 s s) \<and> (Inv_1 s s)))) \<or> (((Inv_1 s s) \<and> (\<not> (finale s))) \<and> ((t1_0 s) > 0))) \<or> (((finalt = 0) \<and> ((reaction_1 s s) \<and> (Inv_1 s s))) \<or> (((Inv_1 s s) \<and> (\<not> (finale s))) \<and> (((t1_1_0 s) = 0) \<and> ((t2_1_0 s) > 0)))))))) \<Longrightarrow>
+EDTL_final_nontemporal_or_tau_delay_true_inv finalt t1_0 t1_1_0 t2_1_0 trigger finale release_1 Inv_1 reaction_1 s"
+
+unfolding EDTL_final_nontemporal_or_tau_delay_true_inv_def
+apply(erule always_rule)
+  apply simp
+  apply(erule conjE)
+  subgoal premises prems1
+  apply(rule conjI)
+  apply(insert prems1(1,2))[1]
+    apply(rule always_disj_rule)
+    apply simp
+      apply(erule conjE)
+      subgoal premises prems2
+      apply(rule conjI)
+      apply(insert prems2(1,2))[1]
+        apply(rule always_imp_refl)
+      apply(insert prems2(1,3))
+        apply(rule always_disj_rule)
+        apply simp
+          apply(erule conjE)
+          subgoal premises prems3
+          apply(rule conjI)
+          apply(insert prems3(1,2))[1]
+            apply simp
+          apply(insert prems3(1,3))
+            apply(rule always_disj_rule)
+            apply simp
+              apply(erule conjE)
+              subgoal premises prems4
+              apply(rule conjI)
+              apply(insert prems4(1,2))[1]
+                apply(rule constrained_until_rule)
+                apply simp
+                  apply(erule conjE)
+                  subgoal premises prems5
+                  apply(rule conjI)
+                  apply(insert prems5(1,2))[1]
+                    apply(rule always_conj_rule)
+                    apply simp
+                      apply(erule conjE)
+                      subgoal premises prems6
+                      apply(rule conjI)
+                      apply(insert prems6(1,2))[1]
+                        apply simp
+                      apply(insert prems6(1,3))
+                        apply(rule always_imp_refl)
+                      done
+                  apply(insert prems5(1,3))
+                    apply(erule conjE)
+                    subgoal premises prems7
+                    apply(rule conjI)
+                    apply(insert prems7(1,2))[1]
+                      apply(rule always_disj_rule)
+                      apply simp
+                        apply(erule conjE)
+                        subgoal premises prems8
+                        apply(rule conjI)
+                        apply(insert prems8(1,2))[1]
+                          apply simp
+                        apply(insert prems8(1,3))
+                          apply(rule always_conj_rule)
+                          apply simp
+                            apply(erule conjE)
+                            subgoal premises prems9
+                            apply(rule conjI)
+                            apply(insert prems9(1,2))[1]
+                              apply(rule always_imp_refl)
+                            apply(insert prems9(1,3))
+                              apply(rule always_conj_rule)
+                              apply simp
+                                apply(erule conjE)
+                                subgoal premises prems10
+                                apply(rule conjI)
+                                apply(insert prems10(1,2))[1]
+                                  apply simp
+                                apply(insert prems10(1,3))
+                                  apply simp
+                                done
+                            done
+                        done
+                    apply(insert prems7(1,3))
+                      apply(erule disjE)
+                      apply(rule disjI1)
+                        apply simp
+                      apply(rule disjI2)
+                        apply(erule disjE)
+                        apply(rule disjI1)
+                          apply(erule conjE)
+                          subgoal premises prems11
+                          apply(rule conjI)
+                          apply(insert prems11(1,2))[1]
+                            apply(erule disjE)
+                            apply(rule disjI1)
+                              apply simp
+                            apply(rule disjI2)
+                              apply(erule conjE)
+                              subgoal premises prems12
+                              apply(rule conjI)
+                              apply(insert prems12(1,2))[1]
+                                apply simp
+                              apply(insert prems12(1,3))
+                                apply(erule conjE)
+                                subgoal premises prems13
+                                apply(rule conjI)
+                                apply(insert prems13(1,2))[1]
+                                  apply simp
+                                apply(insert prems13(1,3))
+                                  apply simp
+                                done
+                              done
+                          apply(insert prems11(1,3))
+                            apply simp
+                          done
+                        apply(rule disjI2)
+                          apply(erule conjE)
+                          subgoal premises prems14
+                          apply(rule conjI)
+                          apply(insert prems14(1,2))[1]
+                            apply(erule conjE)
+                            subgoal premises prems15
+                            apply(rule conjI)
+                            apply(insert prems15(1,2))[1]
+                              apply simp
+                            apply(insert prems15(1,3))
+                              apply simp
+                            done
+                          apply(insert prems14(1,3))
+                            apply simp
+                          done
+                    done
+                  done
+              apply(insert prems4(1,3))
+                apply(rule constrained_until2_rule)
+                apply simp
+                  apply(erule conjE)
+                  subgoal premises prems16
+                  apply(rule conjI)
+                  apply(insert prems16(1,2))[1]
+                    apply(rule always_conj_rule)
+                    apply simp
+                      apply(erule conjE)
+                      subgoal premises prems17
+                      apply(rule conjI)
+                      apply(insert prems17(1,2))[1]
+                        apply simp
+                      apply(insert prems17(1,3))
+                        apply(rule always_imp_refl)
+                      done
+                  apply(insert prems16(1,3))
+                    apply(erule conjE)
+                    subgoal premises prems18
+                    apply(rule conjI)
+                    apply(insert prems18(1,2))[1]
+                      apply(rule always_conj_rule)
+                      apply simp
+                        apply(erule conjE)
+                        subgoal premises prems19
+                        apply(rule conjI)
+                        apply(insert prems19(1,2))[1]
+                          apply simp
+                        apply(insert prems19(1,3))
+                          apply simp
+                        done
+                    apply(insert prems18(1,3))
+                      apply(erule disjE)
+                      apply(rule disjI1)
+                        apply simp
+                      apply(rule disjI2)
+                        apply(erule disjE)
+                        apply(rule disjI1)
+                          apply simp
+                        apply(rule disjI2)
+                          apply(erule disjE)
+                          apply(rule disjI1)
+                            apply(erule conjE)
+                            subgoal premises prems20
+                            apply(rule conjI)
+                            apply(insert prems20(1,2))[1]
+                              apply(erule conjE)
+                              subgoal premises prems21
+                              apply(rule conjI)
+                              apply(insert prems21(1,2))[1]
+                                apply simp
+                              apply(insert prems21(1,3))
+                                apply simp
+                              done
+                            apply(insert prems20(1,3))
+                              apply(erule conjE)
+                              subgoal premises prems22
+                              apply(rule conjI)
+                              apply(insert prems22(1,2))[1]
+                                apply simp
+                              apply(insert prems22(1,3))
+                                apply simp
+                              done
+                            done
+                          apply(rule disjI2)
+                            apply(erule conjE)
+                            subgoal premises prems23
+                            apply(rule conjI)
+                            apply(insert prems23(1,2))[1]
+                              apply(erule conjE)
+                              subgoal premises prems24
+                              apply(rule conjI)
+                              apply(insert prems24(1,2))[1]
+                                apply simp
+                              apply(insert prems24(1,3))
+                                apply simp
+                              done
+                            apply(insert prems23(1,3))
+                              apply(erule conjE)
+                              subgoal premises prems25
+                              apply(rule conjI)
+                              apply(insert prems25(1,2))[1]
+                                apply simp
+                              apply(insert prems25(1,3))
+                                apply simp
+                              done
+                            done
+                    done
+                  done
+              done
+          done
+      done
+  apply(insert prems1(1,3))
+    apply(erule disjE)
+    apply(rule disjI1)
+      apply simp
+    apply(rule disjI2)
+      apply(erule disjE)
+      apply(rule disjI1)
+        apply simp
+      apply(rule disjI2)
+        apply(erule disjE)
+        apply(rule disjI1)
+          apply(rule constrained_until_one_point)
+          apply simp
+            apply(erule disjE)
+            apply(rule disjI1)
+              apply(erule disjE)
+              apply(rule disjI1)
+                apply simp
+              apply(rule disjI2)
+                apply(erule conjE)
+                subgoal premises prems26
+                apply(rule conjI)
+                apply(insert prems26(1,2))[1]
+                  apply simp
+                apply(insert prems26(1,3))
+                  apply(erule conjE)
+                  subgoal premises prems27
+                  apply(rule conjI)
+                  apply(insert prems27(1,2))[1]
+                    apply simp
+                  apply(insert prems27(1,3))
+                    apply simp
+                  done
+                done
+            apply(rule disjI2)
+              apply(erule conjE)
+              subgoal premises prems28
+              apply(rule conjI)
+              apply(insert prems28(1,2))[1]
+                apply(erule conjE)
+                subgoal premises prems29
+                apply(rule conjI)
+                apply(insert prems29(1,2))[1]
+                  apply simp
+                apply(insert prems29(1,3))
+                  apply simp
+                done
+              apply(insert prems28(1,3))
+                apply simp
+              done
+        apply(rule disjI2)
+          apply(rule constrained_until2_one_point)
+          apply simp
+            apply(erule disjE)
+            apply(rule disjI1)
+              apply(erule conjE)
+              subgoal premises prems30
+              apply(rule conjI)
+              apply(insert prems30(1,2))[1]
+                apply simp
+              apply(insert prems30(1,3))
+                apply(erule conjE)
+                subgoal premises prems31
+                apply(rule conjI)
+                apply(insert prems31(1,2))[1]
+                  apply simp
+                apply(insert prems31(1,3))
+                  apply simp
+                done
+              done
+            apply(rule disjI2)
+              apply(erule conjE)
+              subgoal premises prems32
+              apply(rule conjI)
+              apply(insert prems32(1,2))[1]
+                apply(erule conjE)
+                subgoal premises prems33
+                apply(rule conjI)
+                apply(insert prems33(1,2))[1]
+                  apply simp
+                apply(insert prems33(1,3))
+                  apply simp
+                done
+              apply(insert prems32(1,3))
+                apply(erule conjE)
+                subgoal premises prems34
+                apply(rule conjI)
+                apply(insert prems34(1,2))[1]
+                  apply simp
+                apply(insert prems34(1,3))
+                  apply simp
+                done
+              done
+  done
+done
+
+lemma EDTL_final_nontemporal_or_tau_delay_trueeinv_imp_req_gen: "
+EDTL_final_nontemporal_or_tau_delay_true_inv finalt t1_0 t1_1_0 t2_1_0 trigger finale release_1 Inv_1 reaction_1 s0 \<Longrightarrow>
+toEnvP s0 \<Longrightarrow>
+(True \<and> ((always_imp s0 (\<lambda> r1 . (release_1 s0 r1)) (\<lambda> r1 . (release s0 r1))) \<and> ((((always_imp s0 (\<lambda> r3 . (Inv_1 s0 r3)) (\<lambda> r3 . (Inv s0 r3))) \<and> True) \<and> (((always_imp s0 (\<lambda> r3 . (release_1 s0 r3)) (\<lambda> r3 . (release s0 r3))) \<and> (True \<and> ((always_imp s0 (\<lambda> r3 . (reaction_1 s0 r3)) (\<lambda> r3 . (reaction s0 r3))) \<and> (always_imp s0 (\<lambda> r3 . (Inv_1 s0 r3)) (\<lambda> r3 . (Inv s0 r3)))))) \<and> ((t1_0 s0) <= finalt))) \<and> (((always_imp s0 (\<lambda> r3 . (Inv_1 s0 r3)) (\<lambda> r3 . (Inv s0 r3))) \<and> True) \<and> (((always_imp s0 (\<lambda> r3 . (reaction_1 s0 r3)) (\<lambda> r3 . (reaction s0 r3))) \<and> (always_imp s0 (\<lambda> r3 . (Inv_1 s0 r3)) (\<lambda> r3 . (Inv s0 r3)))) \<and> ((t2_1_0 s0) <= finalt)))))) \<Longrightarrow>
+EDTL_final_nontemporal_or_tau_delay_true finalt trigger finale release Inv reaction s0"
+
+unfolding EDTL_final_nontemporal_or_tau_delay_true_inv_def EDTL_final_nontemporal_or_tau_delay_true_def
+apply(erule always_einv2req)
+apply simp
+  apply(rule always_disj_rule)
+  apply simp
+    apply(erule conjE)
+    subgoal premises prems3
+    apply(rule conjI)
+    apply(insert prems3(1,2))[1]
+      apply(rule always_imp_refl)
+    apply(insert prems3(1,3))
+      apply(rule always_disj_rule)
+      apply simp
+        apply(erule conjE)
+        subgoal premises prems4
+        apply(rule conjI)
+        apply(insert prems4(1,2))[1]
+          apply simp
+        apply(insert prems4(1,3))
+          apply(rule always_disj_rule)
+          apply simp
+            apply(erule conjE)
+            subgoal premises prems5
+            apply(rule conjI)
+            apply(insert prems5(1,2))[1]
+              apply(rule constrained_until_einv2req)
+              apply simp
+                apply(erule conjE)
+                subgoal premises prems6
+                apply(rule conjI)
+                apply(insert prems6(1,2))[1]
+                  apply(rule always_conj_rule)
+                  apply simp
+                    apply(erule conjE)
+                    subgoal premises prems7
+                    apply(rule conjI)
+                    apply(insert prems7(1,2))[1]
+                      apply simp
+                    apply(insert prems7(1,3))
+                      apply(rule always_imp_refl)
+                    done
+                apply(insert prems6(1,3))
+                  apply(erule conjE)
+                  subgoal premises prems8
+                  apply(rule conjI)
+                  apply(insert prems8(1,2))[1]
+                    apply(rule always_disj_rule)
+                    apply simp
+                      apply(erule conjE)
+                      subgoal premises prems9
+                      apply(rule conjI)
+                      apply(insert prems9(1,2))[1]
+                        apply simp
+                      apply(insert prems9(1,3))
+                        apply(rule always_conj_rule)
+                        apply simp
+                          apply(erule conjE)
+                          subgoal premises prems10
+                          apply(rule conjI)
+                          apply(insert prems10(1,2))[1]
+                            apply(rule always_imp_refl)
+                          apply(insert prems10(1,3))
+                            apply(rule always_conj_rule)
+                            apply simp
+                              apply(erule conjE)
+                              subgoal premises prems11
+                              apply(rule conjI)
+                              apply(insert prems11(1,2))[1]
+                                apply simp
+                              apply(insert prems11(1,3))
+                                apply simp
+                              done
+                          done
+                      done
+                  apply(insert prems8(1,3))
+                    apply simp
+                  done
+                done
+            apply(insert prems5(1,3))
+              apply(rule constrained_until2_einv2req)
+              apply simp
+                apply(erule conjE)
+                subgoal premises prems12
+                apply(rule conjI)
+                apply(insert prems12(1,2))[1]
+                  apply(rule always_conj_rule)
+                  apply simp
+                    apply(erule conjE)
+                    subgoal premises prems13
+                    apply(rule conjI)
+                    apply(insert prems13(1,2))[1]
+                      apply simp
+                    apply(insert prems13(1,3))
+                      apply(rule always_imp_refl)
+                    done
+                apply(insert prems12(1,3))
+                  apply(erule conjE)
+                  subgoal premises prems14
+                  apply(rule conjI)
+                  apply(insert prems14(1,2))[1]
+                    apply(rule always_conj_rule)
+                    apply simp
+                      apply(erule conjE)
+                      subgoal premises prems15
+                      apply(rule conjI)
+                      apply(insert prems15(1,2))[1]
+                        apply simp
+                      apply(insert prems15(1,3))
+                        apply simp
+                      done
+                  apply(insert prems14(1,3))
+                    apply simp
+                  done
+                done
+            done
+        done
+    done
+done
+
+lemma EDTL_final_nontemporal_or_tau_delay_true_inv_saving: "
+EDTL_final_nontemporal_or_tau_delay_true_inv_part finalt t1_0 t1_1_0 t2_1_0 trigger finale release Inv reaction s0 \<Longrightarrow>
+consecutive s0 s \<Longrightarrow>
+(((((t1_0 s0) = 0) \<or> ((((release s) \<or> ((finale s) \<and> ((reaction s) \<and> (Inv s)))) \<and> ((t1_0 s0) <= finalt)) \<or> (((Inv s) \<and> (\<not> (finale s))) \<and> ((t1_0 s0) < (t1_0 s))))) \<and> (((t2_1_0 s0) = 0) \<or> (((t1_1_0 s0) >= (t2_1_0 s0)) \<or> ((((reaction s) \<and> (Inv s)) \<and> ((((t1_1_0 s0) + 1) >= finalt) \<and> ((t2_1_0 s0) <= finalt))) \<or> (((Inv s) \<and> (\<not> (finale s))) \<and> ((((t1_1_0 s0) + 1) >= (t1_1_0 s)) \<and> ((t2_1_0 s0) < (t2_1_0 s)))))))) \<and> ((\<not> (trigger s)) \<or> ((release s) \<or> ((((release s) \<or> ((finale s) \<and> ((reaction s) \<and> (Inv s)))) \<or> (((Inv s) \<and> (\<not> (finale s))) \<and> ((t1_0 s) > 0))) \<or> (((finalt = 0) \<and> ((reaction s) \<and> (Inv s))) \<or> (((Inv s) \<and> (\<not> (finale s))) \<and> (((t1_1_0 s) = 0) \<and> ((t2_1_0 s) > 0)))))))) \<Longrightarrow>
+EDTL_final_nontemporal_or_tau_delay_true_inv_part finalt t1_0 t1_1_0 t2_1_0 trigger finale release Inv reaction s"
+
+unfolding EDTL_final_nontemporal_or_tau_delay_true_inv_part_def EDTL_final_nontemporal_or_tau_delay_true_part_def
+apply(simp add: EDTL_final_nontemporal_or_tau_delay_true_inv_saving_gen always_imp_refl)
+done
+
+lemma EDTL_final_nontemporal_or_tau_delay_trueeinv_imp_req: "
+EDTL_final_nontemporal_or_tau_delay_true_inv_part finalt t1_0 t1_1_0 t2_1_0 trigger finale release Inv reaction s \<Longrightarrow>
+toEnvP s \<Longrightarrow>
+(((t1_0 s) <= finalt) \<and> ((t2_1_0 s) <= finalt)) \<Longrightarrow>
+EDTL_final_nontemporal_or_tau_delay_true_part finalt trigger finale release Inv reaction s"
+
+unfolding EDTL_final_nontemporal_or_tau_delay_true_inv_part_def EDTL_final_nontemporal_or_tau_delay_true_part_def
+apply(simp add: EDTL_final_nontemporal_or_tau_delay_trueeinv_imp_req_gen always_imp_refl)
+done
+
+
+
+lemmas EDTL_final_nontemporal_or_tau_delay_true_used_patterns = EDTL_final_nontemporal_or_tau_delay_true_def always_used_patterns constrained_until_def constrained_until2_def 
+
+lemmas EDTL_final_nontemporal_or_tau_delay_true_inv_used_patterns = EDTL_final_nontemporal_or_tau_delay_true_inv_def always_inv_used_patterns constrained_until_inv_def constrained_until2_inv_def 
+
+lemmas EDTL_final_nontemporal_or_tau_delay_true_inv_part_used_patterns = EDTL_final_nontemporal_or_tau_delay_true_inv_part_def EDTL_final_nontemporal_or_tau_delay_true_inv_used_patterns
+
+lemmas EDTL_final_nontemporal_or_tau_delay_true_part_used_patterns = EDTL_final_nontemporal_or_tau_delay_true_part_def EDTL_final_nontemporal_or_tau_delay_true_used_patterns
+
+definition EDTL_release_false_final_tau_delay_tau where "EDTL_release_false_final_tau_delay_tau fin delay trigger Inv reaction s \<equiv> (always (\<lambda> r2 r1 . ((\<not> (trigger r1)) \<or> (constrained_until2 fin (fin + delay) Inv (\<lambda> r4 r3 . ((reaction r4 r3) \<and> (Inv r4 r3))) r2 r1))) s)"
+
+definition EDTL_release_false_final_tau_delay_tau_part where "EDTL_release_false_final_tau_delay_tau_part fin delay trigger Inv reaction s \<equiv> (EDTL_release_false_final_tau_delay_tau fin delay trigger (\<lambda> s s1 . (Inv s1)) (\<lambda> s s1 . (reaction s1)) s)"
+
+definition EDTL_release_false_final_tau_delay_tau_inv where "EDTL_release_false_final_tau_delay_tau_inv fin delay t1_1_0 t2_1_0 trigger Inv_1 reaction_1 s \<equiv> (always_inv (\<lambda> r2 r1 . ((\<not> (trigger r1)) \<or> (constrained_until2_inv fin (fin + delay) t1_1_0 t2_1_0 Inv_1 (\<lambda> r4 r3 . ((reaction_1 r4 r3) \<and> (Inv_1 r4 r3))) r2 r1))) s)"
+
+definition EDTL_release_false_final_tau_delay_tau_inv_part where "EDTL_release_false_final_tau_delay_tau_inv_part fin delay t1_1_0 t2_1_0 trigger Inv reaction s \<equiv> (EDTL_release_false_final_tau_delay_tau_inv fin delay t1_1_0 t2_1_0 trigger (\<lambda> s s1 . (Inv s1)) (\<lambda> s s1 . (reaction s1)) s)"
+
+lemma EDTL_release_false_final_tau_delay_tau_inv_saving_gen: "
+EDTL_release_false_final_tau_delay_tau_inv fin delay t1_1_0 t2_1_0 trigger Inv_1 reaction_1 s0 \<Longrightarrow>
+consecutive s0 s \<Longrightarrow>
+((True \<and> ((always_imp s0 (Inv_1 s0) (Inv_1 s)) \<and> (((always_imp s0 (\<lambda> r3 . (reaction_1 s0 r3)) (\<lambda> r3 . (reaction_1 s r3))) \<and> (always_imp s0 (\<lambda> r3 . (Inv_1 s0 r3)) (\<lambda> r3 . (Inv_1 s r3)))) \<and> (((t2_1_0 s0) = 0) \<or> (((t1_1_0 s0) >= (t2_1_0 s0)) \<or> ((((reaction_1 s s) \<and> (Inv_1 s s)) \<and> ((((t1_1_0 s0) + 1) >= fin) \<and> ((t2_1_0 s0) <= (fin + delay)))) \<or> ((Inv_1 s s) \<and> ((((t1_1_0 s0) + 1) >= (t1_1_0 s)) \<and> ((t2_1_0 s0) < (t2_1_0 s)))))))))) \<and> ((\<not> (trigger s)) \<or> (((fin = 0) \<and> ((reaction_1 s s) \<and> (Inv_1 s s))) \<or> ((Inv_1 s s) \<and> (((t1_1_0 s) = 0) \<and> ((t2_1_0 s) > 0)))))) \<Longrightarrow>
+EDTL_release_false_final_tau_delay_tau_inv fin delay t1_1_0 t2_1_0 trigger Inv_1 reaction_1 s"
+
+unfolding EDTL_release_false_final_tau_delay_tau_inv_def
+apply(erule always_rule)
+  apply simp
+  apply(erule conjE)
+  subgoal premises prems1
+  apply(rule conjI)
+  apply(insert prems1(1,2))[1]
+    apply(rule always_disj_rule)
+    apply simp
+      apply(erule conjE)
+      subgoal premises prems2
+      apply(rule conjI)
+      apply(insert prems2(1,2))[1]
+        apply(rule always_imp_refl)
+      apply(insert prems2(1,3))
+        apply(rule constrained_until2_rule)
+        apply simp
+          apply(erule conjE)
+          subgoal premises prems3
+          apply(rule conjI)
+          apply(insert prems3(1,2))[1]
+            apply simp
+          apply(insert prems3(1,3))
+            apply(erule conjE)
+            subgoal premises prems4
+            apply(rule conjI)
+            apply(insert prems4(1,2))[1]
+              apply(rule always_conj_rule)
+              apply simp
+                apply(erule conjE)
+                subgoal premises prems5
+                apply(rule conjI)
+                apply(insert prems5(1,2))[1]
+                  apply simp
+                apply(insert prems5(1,3))
+                  apply simp
+                done
+            apply(insert prems4(1,3))
+              apply(erule disjE)
+              apply(rule disjI1)
+                apply simp
+              apply(rule disjI2)
+                apply(erule disjE)
+                apply(rule disjI1)
+                  apply simp
+                apply(rule disjI2)
+                  apply(erule disjE)
+                  apply(rule disjI1)
+                    apply(erule conjE)
+                    subgoal premises prems6
+                    apply(rule conjI)
+                    apply(insert prems6(1,2))[1]
+                      apply(erule conjE)
+                      subgoal premises prems7
+                      apply(rule conjI)
+                      apply(insert prems7(1,2))[1]
+                        apply simp
+                      apply(insert prems7(1,3))
+                        apply simp
+                      done
+                    apply(insert prems6(1,3))
+                      apply(erule conjE)
+                      subgoal premises prems8
+                      apply(rule conjI)
+                      apply(insert prems8(1,2))[1]
+                        apply simp
+                      apply(insert prems8(1,3))
+                        apply simp
+                      done
+                    done
+                  apply(rule disjI2)
+                    apply(erule conjE)
+                    subgoal premises prems9
+                    apply(rule conjI)
+                    apply(insert prems9(1,2))[1]
+                      apply simp
+                    apply(insert prems9(1,3))
+                      apply(erule conjE)
+                      subgoal premises prems10
+                      apply(rule conjI)
+                      apply(insert prems10(1,2))[1]
+                        apply simp
+                      apply(insert prems10(1,3))
+                        apply simp
+                      done
+                    done
+            done
+          done
+      done
+  apply(insert prems1(1,3))
+    apply(erule disjE)
+    apply(rule disjI1)
+      apply simp
+    apply(rule disjI2)
+      apply(rule constrained_until2_one_point)
+      apply simp
+        apply(erule disjE)
+        apply(rule disjI1)
+          apply(erule conjE)
+          subgoal premises prems11
+          apply(rule conjI)
+          apply(insert prems11(1,2))[1]
+            apply simp
+          apply(insert prems11(1,3))
+            apply(erule conjE)
+            subgoal premises prems12
+            apply(rule conjI)
+            apply(insert prems12(1,2))[1]
+              apply simp
+            apply(insert prems12(1,3))
+              apply simp
+            done
+          done
+        apply(rule disjI2)
+          apply(erule conjE)
+          subgoal premises prems13
+          apply(rule conjI)
+          apply(insert prems13(1,2))[1]
+            apply simp
+          apply(insert prems13(1,3))
+            apply(erule conjE)
+            subgoal premises prems14
+            apply(rule conjI)
+            apply(insert prems14(1,2))[1]
+              apply simp
+            apply(insert prems14(1,3))
+              apply simp
+            done
+          done
+  done
+done
+
+lemma EDTL_release_false_final_tau_delay_taueinv_imp_req_gen: "
+EDTL_release_false_final_tau_delay_tau_inv fin delay t1_1_0 t2_1_0 trigger Inv_1 reaction_1 s0 \<Longrightarrow>
+toEnvP s0 \<Longrightarrow>
+(True \<and> ((always_imp s0 (Inv_1 s0) (Inv s0)) \<and> (((always_imp s0 (\<lambda> r3 . (reaction_1 s0 r3)) (\<lambda> r3 . (reaction s0 r3))) \<and> (always_imp s0 (\<lambda> r3 . (Inv_1 s0 r3)) (\<lambda> r3 . (Inv s0 r3)))) \<and> ((t2_1_0 s0) <= (fin + delay))))) \<Longrightarrow>
+EDTL_release_false_final_tau_delay_tau fin delay trigger Inv reaction s0"
+
+unfolding EDTL_release_false_final_tau_delay_tau_inv_def EDTL_release_false_final_tau_delay_tau_def
+apply(erule always_einv2req)
+apply simp
+  apply(rule always_disj_rule)
+  apply simp
+    apply(erule conjE)
+    subgoal premises prems3
+    apply(rule conjI)
+    apply(insert prems3(1,2))[1]
+      apply(rule always_imp_refl)
+    apply(insert prems3(1,3))
+      apply(rule constrained_until2_einv2req)
+      apply simp
+        apply(erule conjE)
+        subgoal premises prems4
+        apply(rule conjI)
+        apply(insert prems4(1,2))[1]
+          apply simp
+        apply(insert prems4(1,3))
+          apply(erule conjE)
+          subgoal premises prems5
+          apply(rule conjI)
+          apply(insert prems5(1,2))[1]
+            apply(rule always_conj_rule)
+            apply simp
+              apply(erule conjE)
+              subgoal premises prems6
+              apply(rule conjI)
+              apply(insert prems6(1,2))[1]
+                apply simp
+              apply(insert prems6(1,3))
+                apply simp
+              done
+          apply(insert prems5(1,3))
+            apply simp
+          done
+        done
+    done
+done
+
+lemma EDTL_release_false_final_tau_delay_tau_inv_saving: "
+EDTL_release_false_final_tau_delay_tau_inv_part fin delay t1_1_0 t2_1_0 trigger Inv reaction s0 \<Longrightarrow>
+consecutive s0 s \<Longrightarrow>
+((((t2_1_0 s0) = 0) \<or> (((t1_1_0 s0) >= (t2_1_0 s0)) \<or> ((((reaction s) \<and> (Inv s)) \<and> ((((t1_1_0 s0) + 1) >= fin) \<and> ((t2_1_0 s0) <= (fin + delay)))) \<or> ((Inv s) \<and> ((((t1_1_0 s0) + 1) >= (t1_1_0 s)) \<and> ((t2_1_0 s0) < (t2_1_0 s))))))) \<and> ((\<not> (trigger s)) \<or> (((fin = 0) \<and> ((reaction s) \<and> (Inv s))) \<or> ((Inv s) \<and> (((t1_1_0 s) = 0) \<and> ((t2_1_0 s) > 0)))))) \<Longrightarrow>
+EDTL_release_false_final_tau_delay_tau_inv_part fin delay t1_1_0 t2_1_0 trigger Inv reaction s"
+
+unfolding EDTL_release_false_final_tau_delay_tau_inv_part_def EDTL_release_false_final_tau_delay_tau_part_def
+apply(simp add: EDTL_release_false_final_tau_delay_tau_inv_saving_gen always_imp_refl)
+done
+
+lemma EDTL_release_false_final_tau_delay_taueinv_imp_req: "
+EDTL_release_false_final_tau_delay_tau_inv_part fin delay t1_1_0 t2_1_0 trigger Inv reaction s \<Longrightarrow>
+toEnvP s \<Longrightarrow>
+((t2_1_0 s) <= (fin + delay)) \<Longrightarrow>
+EDTL_release_false_final_tau_delay_tau_part fin delay trigger Inv reaction s"
+
+unfolding EDTL_release_false_final_tau_delay_tau_inv_part_def EDTL_release_false_final_tau_delay_tau_part_def
+apply(simp add: EDTL_release_false_final_tau_delay_taueinv_imp_req_gen always_imp_refl)
+done
+
+
+
+lemmas EDTL_release_false_final_tau_delay_tau_used_patterns = EDTL_release_false_final_tau_delay_tau_def always_used_patterns constrained_until2_def 
+
+lemmas EDTL_release_false_final_tau_delay_tau_inv_used_patterns = EDTL_release_false_final_tau_delay_tau_inv_def always_inv_used_patterns constrained_until2_inv_def 
+
+lemmas EDTL_release_false_final_tau_delay_tau_inv_part_used_patterns = EDTL_release_false_final_tau_delay_tau_inv_part_def EDTL_release_false_final_tau_delay_tau_inv_used_patterns
+
+lemmas EDTL_release_false_final_tau_delay_tau_part_used_patterns = EDTL_release_false_final_tau_delay_tau_part_def EDTL_release_false_final_tau_delay_tau_used_patterns
+
+end
